Safer list insert, preapring non initialized memory check

AbstractMemory.v
@@ -1,64 +1,88 @@
 Require Import MachineInt.
 Require Import List.
-Require Import Repeat.
+Require Import Insert.
 
 Module AbstractMemory.
 
 Module Context.
 
+Parameter nb_memories : nat.
+
 End Context.
 
 Definition Mem := list byte.
 
-Definition Inv_1 (B: Mem) : Prop := True.
+Definition Guard (l: nat) : Prop := l >= 0 /\ l < Context.nb_memories.
+
+Module Init.
+Definition Guard (limit:nat) : Prop := Context.nb_memories = limit.
+End Init.
 
 Module Store.
 
-Fixpoint replace_at {A:Set} (l: list A) (n : nat) (elt : A) : list A :=
-    match l, n with
-    | nil, _ => elt::nil
-    | h :: t, 0 => elt::t 
-    | h :: t, S n' => h :: replace_at t n' elt
-    end.
+(*
+Lemma belong: forall A : Set, forall l1 l2 l3 : list A, forall e : A, forall n : nat,
+app l2 l3 = l1
+-> l2 = firstn n l1 -> l3 = skipn n l1
+-> (length l2 = n /\ length l3 = (length l1 - n) /\ length l1 >= 0 /\  n < length l1) 
+-> replace_at l1 n e = app l2 (e::l3).
+intros A l1 l2 l3 e n.
+simpl.
+intros H1 H2 H3 H4.
 
-Definition store8 (M : Mem) (l : nat) (b : byte) : Mem := replace_at M l b.
+induction l1 as [|x lx].
++simpl.
+rewrite app_eq_nil in H1.
+inversion H1.
+*)
 
-Definition Guard : Prop := True.
-Definition action (S : Mem) (l : nat) (b : byte) : Mem := store8 S l b.
+Definition Inv_1 (M: option Mem) : Prop := True.
 
-Lemma PO_Safety: forall S: Mem, Guard -> let S' := action in Inv_1 S.
-intros S.
+Definition store8 (M : Mem) (l : nat) (b : byte) : option Mem := replace_at M l b.
+
+Definition action (S : Mem) (l : nat) (b : byte) : option Mem := store8 S l b.
+
+Lemma PO_Safety: forall S: Mem, forall l: nat, forall b: byte, Init.Guard 4096 -> Guard l -> let S' := action S l b in Inv_1 S'.
+intros S l b.
 simpl.
 compute.
 intro.
-exact H.
+rewrite H.
+split.
 Qed.
 
 End Store.
 
 Module Load.
 
-Definition load8 (M : Mem) (l : nat) : option byte :=
+Definition Inv_1 (b: byte) : Prop := True.
+
+Definition load8 (M : Mem) (l : nat) : byte :=
     match skipn l M with
-    | nil => None
-    | h :: t => Some h
+    | nil => Byte.repr 0
+    | h :: t => h
     end.
 
-Definition Guard : Prop := True.
-Definition action (S : Mem) (l : nat) : byte :=
-    match load8 S l with
-    | None => Byte.repr 0
-    | Some b => b
-    end.
+Definition action (S : Mem) (l : nat) : byte := load8 S l.
 
-Lemma PO_Safety: forall S: Mem, Guard -> let S' := action in Inv_1 S.
-intros S.
-simpl.
+Lemma PO_Safety: forall S: Mem, forall l: nat, Init.Guard 4096 -> Guard l -> let b' := action S l in Inv_1 b'.
+intros S l.
 compute.
-intro.
-exact H.
+intro H.
+rewrite H.
+split.
 Qed.
 
 End Load.
+
+(*
+Lemma load_store_eq_8 :
+  forall (M : Mem) (l : nat) (b : byte), Load.load8 (Store.store8 M l b) l = b.
+intros S l b.
+unfold Store.store8.
+unfold Store.replace_at.
+compute.
+simpl.
+*)
 
 End AbstractMemory.
