Insert.v
@@ -1,0 +1,41 @@
+Require Import Arith.
+Require Import List.
+Import ListNotations.
+
+Lemma zltz: 0 < 0 -> False.
+Proof.
+  intros. contradict H. apply Lt.lt_irrefl.
+Qed.
+
+Lemma nltz: forall n: nat, n < 0 -> False.
+Proof.
+  intros. contradict H. apply Lt.lt_n_0.
+Qed.
+
+Lemma predecessor_proof: forall {X: Type} (n: nat) (x: X) (xs: list X),
+  S n < length (x::xs) -> n < length xs.
+Proof.
+  intros. simpl in H. apply Lt.lt_S_n. assumption.
+Qed.
+
+Fixpoint safe_nth' {X: Type} (xs: list X) (n: nat): n < length xs -> X :=
+  match xs, n with
+  | [], _ => fun pf => match nltz n pf with end
+  | x::_, 0 => fun _ => x
+  | x::xs', S n' => fun pf => safe_nth' xs' n' (predecessor_proof n' x xs' pf)
+  end.
+
+Fixpoint safe_insert {X: Type} (xs: list X) (n: nat) (elt: X): n < length xs -> list X :=
+  match xs, n with
+    | nil, _ => fun pf => elt::nil
+    | h::t, 0 => fun _ => elt::t
+    | h :: t, S n' => fun pf => h :: safe_insert t n' elt (predecessor_proof n' h t pf)
+    end.
+
+Definition replace_at {A:Type} (l: list A) (n : nat) (elt : A)  :=
+match lt_dec n (length l) with
+  | left pf => Some (safe_insert l n elt pf)
+  | right _ => None
+  end.
+
+Eval compute in replace_at [1;2;3] 0 4.
