Main.v
@@ -15,13 +15,13 @@ Inductive outcome: Type :=
 
 Definition exec_load (a: nat) (dest: AbstractRegister.Reg8) (S: State) :=
   match AbstractMemory.Load.load8 (_M S) a with
-  | Some v => Next (nextinstr (AbstractRegister.SetRegister.setReg8 (_R S) dest v, _M S, _PC S, _ST S))
-  | None => Stuck
+  | v => Next (nextinstr (AbstractRegister.SetRegister.setReg8 (_R S) dest v, _M S, _PC S, _ST S))
   end.
 
 Definition exec_store (a: nat) (S: State) (source: AbstractRegister.Reg8) :=
   match AbstractMemory.Store.store8 (_M S) a (AbstractRegister.GetRegisterValue.getReg8 (_R S) source) with
-  | m' => Next (nextinstr (_R S, m', _PC S, _ST S))
+  | Some m' => Next (nextinstr (_R S, m', _PC S, _ST S))
+  | None => Stuck
   end.
 
 Definition exec_load_imm (b: byte) (S : State) (R : AbstractRegister.Reg8) :=
@@ -45,7 +45,7 @@ end.
 
 Definition StartR : AbstractRegister.RegF := AbstractRegister.mkState (Byte.repr 0) (Byte.repr 0) (Byte.repr 0).
 
-Definition StartM : AbstractMemory.Mem := repeat (Byte.repr 0) 64.
+Definition StartM : AbstractMemory.Mem := repeat (Byte.repr 0) 4096.
 
 Definition StartPC : word := Word.repr 0.
 
@@ -78,8 +78,6 @@ Fixpoint step (S1 : State) (p: list Instr) : option State :=
         | None => None
         end.
 
-Eval simpl in step StartP prog1.
-
 Fixpoint run (S1 : State) (p: list Instr) (n : nat) : State :=
   match n with
   | 0%nat => S1
@@ -89,4 +87,4 @@ Fixpoint run (S1 : State) (p: list Instr) (n : nat) : State :=
               end
 end.
 
-Eval compute in run StartP prog1 (length prog1).
+Eval compute in run StartP prog1 100.
